A commit just to show a problem with get operator on bitstring in gate.ec

proof/gate.ec
@@ -1,28 +1,35 @@
 require import Bitstring.
 require import Int.
 require import Map.
+require import Pair.
+
 require import Scheme.
+require import Dkc.
+
+cnst unit : unit.
 
 theory Gate.
   clone Scheme as Scheme.
   export Scheme.
 
-  type token = bitstring.
+  type token = Dkc.number.
 
   type funct = bool*bool*bool*bool.
-  type functG = ((bool*bool), token) map.
+  type functG = token*token*token*token.
   type input = bool*bool.
   type output = bool.
   type keyInput = token*token*token*token.
   type keyOutput = unit.
   type inputG = token*token.
-  type outputG = token.
-  
+  type outputG = bool.
+
+  type tokens = (int*bool, Gate.token) map.
+
   type query = (funct*input)*(funct*input).
   type answer = functG*inputG*keyOutput.
   
   op tweak(a:bool, b:bool) : bitstring = a::(b::(zeros (k-2))).
-
+  
   op eval(f:funct, i:input) : output =
     let (ff, ft, tf, tt) = f in
     let (i1, i2) = i in
@@ -30,4 +37,46 @@ theory Gate.
     if (((i1=false) && (i2=true))) then ft else
     if (((i1=true) && (i2=false))) then tf else
     tt.
+
+  op enc(x:tokens, f:funct, x1:bool, x2:bool) : token =
+    Dkc.encode (tweak x1 x2) (proj x.[(1, x1)]) (proj x.[(2, x2)]) (proj x.[(3, eval f (x1,x2))]).
+  op garble(x:tokens, f:funct) : functG*keyInput*keyOutput =
+    (
+      (enc x f false false, enc x f false true, enc x f true false, enc x f true true),
+      (proj x.[(1, false)], proj x.[(1, true)], proj x.[(2, false)], proj x.[(2, true)]),
+      unit
+    ).
+  (*pred tokenCorrect(x:tokens) =
+    (to_array x.[(1, false)]).[0] != (to_array x.[(1, true)]).[0] &&
+    (to_array x.[(2, false)]).[0] != (to_array x.[(2, true)]).[0] &&
+    (to_array x.[(3, false)]).[0] == false &&
+    (to_array x.[(3, false)]).[0] == true.*)
+
+  op encrypt(k:keyInput, i:input) : inputG =
+    let (f1, t1, f2, t2) = k in
+    let x1 = if fst i then t1 else f1 in
+    let x2 = if snd i then t2 else f2 in
+    (x1, x2).
+
+  op decrypt(k:keyOutput, o:outputG) : output = o.
+
+  op evalG(g:functG, i:inputG) : outputG =
+    let (ff, ft, tf, tt) = g in
+    let a = (fst i).[0] in
+    let b = (snd i).[0] in
+    let t =
+      if (a = false) && (b = false) then ff else
+      if (a = false) && (b = true) then ft else
+      if (a = true) && (b = false) then tf else
+      tt in
+    let u = Dkc.decode (tweak a b) (fst i) (snd i) t in
+    u.[0] (* C'est moche mais j'ai pas trouvé d'autre solution, c'est pas terrible*)
+    .
+    
+  lemma inverse :
+    forall (f : funct) ,
+    forall (i : input) ,
+    forall (x : tokens) ,
+      let (g, ki, ko) = garble x f in
+      eval f i = decrypt ko (evalG g (encrypt ki i)).
 end Gate.
